Give a more telling name to the variable containing a proof

Coq/Articles/utilitarian_ethic_no_freedom_iff_maximum_for_unique_action.v
@@ -32,40 +32,42 @@ Qed.
 
 Definition utilitarian_ethic_unique_maximum {ps : PreferenceSpace}
 (ethic : Ethic) (uf : @UtilityFunction ps)
-(p : maximizes ethic uf) (state : State) :=
+(ethic_maximizes_uf : maximizes ethic uf) (state : State) :=
   exists! (action : Action), is_maximum uf state (uf state action).
 
 Definition utilitarian_ethic_always_unique_maximum {ps : PreferenceSpace}
-(ethic : Ethic) (uf : @UtilityFunction ps) (p : maximizes ethic uf) :=
-  forall (state: State), utilitarian_ethic_unique_maximum ethic uf p state.
+(ethic : Ethic) (uf : @UtilityFunction ps) (ethic_maximizes_uf : maximizes ethic uf) :=
+  forall (state: State),
+    utilitarian_ethic_unique_maximum ethic uf ethic_maximizes_uf state.
 
 Proposition utilitarian_ethic_no_freedom_iff_maximum_for_unique_action
 {ps : PreferenceSpace} :
-  forall (ethic: Ethic) (uf : UtilityFunction) (p : maximizes ethic uf) (state: State),
-    @utilitarian_ethic_unique_maximum ps ethic uf p state <->
+  forall (ethic: Ethic) (uf : UtilityFunction)
+  (ethic_maximizes_uf : maximizes ethic uf) (state: State),
+    @utilitarian_ethic_unique_maximum ps ethic uf ethic_maximizes_uf state <->
     leaves_no_freedom ethic state.
 Proof.
   intros.
-  unfold maximizes in p.
+  unfold maximizes in ethic_maximizes_uf.
   split.
   - intro. unfold leaves_no_freedom. unfold unique.
     unfold utilitarian_ethic_unique_maximum in H.
     destruct H. unfold unique in H. destruct H.
     exists x. split.
-    + pose proof (p state). pose proof (H1 x).
+    + pose proof (ethic_maximizes_uf state). pose proof (H1 x).
       rewrite <- H2 in H. unfold Is_true in H.
       destruct (ethic state x).
       { reflexivity. }
       { inversion H. }
     + intros.
       pose proof (H0 x'). apply H2.
-      pose proof (p state). pose proof (H3 x').
+      pose proof (ethic_maximizes_uf state). pose proof (H3 x').
       rewrite <- H4. unfold Is_true.
       rewrite H1. tauto.
   - intro. unfold leaves_no_freedom in H. unfold unique in H.
     unfold utilitarian_ethic_unique_maximum. unfold unique.
     destruct H. destruct H.
-    pose proof (p state).
+    pose proof (ethic_maximizes_uf state).
     exists x. split.
     + pose proof (H1 x).
       rewrite <- H2. rewrite H. easy.
@@ -78,12 +80,14 @@ Qed.
 
 Corollary utilitarian_ethic_never_freedom_iff_always_maximum_for_unique_action
 {ps : PreferenceSpace} :
-  forall (ethic: Ethic) (uf : UtilityFunction) (p : maximizes ethic uf),
-    @utilitarian_ethic_always_unique_maximum ps ethic uf p <-> never_leaves_freedom ethic.
+  forall (ethic: Ethic) (uf : UtilityFunction)
+  (ethic_maximizes_uf : maximizes ethic uf),
+    @utilitarian_ethic_always_unique_maximum ps ethic uf ethic_maximizes_uf <->
+    never_leaves_freedom ethic.
 Proof.
   intros. unfold utilitarian_ethic_always_unique_maximum. unfold never_leaves_freedom.
   split ; intros; pose proof (H state) ; 
   apply @utilitarian_ethic_no_freedom_iff_maximum_for_unique_action with
-  (ps:=ps) (ethic:=ethic) (uf:=uf) (p:=p) ;
+  (ps:=ps) (ethic:=ethic) (uf:=uf) (ethic_maximizes_uf:=ethic_maximizes_uf) ;
   tauto.
 Qed.
